pico-nosubtyping-fullvpa/Notations.v
@@ -1,5 +1,6 @@
 (* ------------------------------------------------------------------------ *)
 (* Adapted from Celsius project : https://github.com/clementblaudeau/celsius *)
+(** ** Non-overloaded notations *)
 
 (* Typing *)
 Reserved Notation "q1 ⊑ q2" (at level 40).
